eIris/proofmode/base.v
@@ -4,6 +4,8 @@ From iris.bi Require Export bi telescopes interface derived_laws.
 Import bi.
 Import env_notations.
 
+From eIris.proofmode Require Import proper.
+
 Section tactics.
 Context {PROP : bi}.
 Implicit Types Γ : env PROP.
@@ -81,6 +83,37 @@ Proof.
   - rewrite intuitionistically_if_elim HP1. destruct Hmod.
     by rewrite assoc wand_elim_l wand_elim_r HQ.
 Qed.
+
+Lemma iproper_top_to_iproper A B R m f :
+  @IProperTop PROP A B R m f →
+  ⊢@{PROP} (f R) m m.
+Proof.
+  intros HIPT.
+  unfold IProperTop in HIPT.
+  done.
+Qed.
+
+(* 
+Lemma tac_pose_proper A B Δ j R m IP P Q :
+  @IProperTop PROP A B R m IP →
+  @IProper PROP B (f R) m →
+  match envs_app true (Esnoc Enil j IP) Δ with
+  | None => False
+  | Some Δ' => envs_entails Δ' Q
+  end →
+  envs_entails Δ Q.
+Proof.
+  destruct (envs_app _ _ _) as [Δ'|] eqn:?; last done.
+  rewrite envs_entails_unseal => HP HIP <-.
+  assert (⊢ IP).
+  { 
+    unfold IProperTop in HP.
+    destruct HP as [f HP].
+    apply HP.
+  }
+  rewrite envs_app_singleton_sound //=.
+  by rewrite -HP /= intuitionistically_emp emp_wand.
+Qed. *)
 
 End tactics.
 
